WIP Typeclass bug

internal/LobsTheoremProof.v
@@ -75,12 +75,24 @@ Module LC <: LobExtendedContext.
   Bind Scope well_typed_term_scope with box'.
 End LC.
 
+Module PRP <: PretermReflectionPrimitives LC.
+  Definition qPreterm := term'.
+  Notation "‘Preterm’" := qPreterm : preterm_scope.
+
+  Definition qquote : LC.Preterm.
+  Proof.
+    let t := (eval cbv beta delta [qO qS qEmptyString qString qnAnon qAscii qnil qcons qmkdef qtInd qtFix qtCase qtUnknown qtRel qtConstruct qtEvar qtMeta qtVar qtApp qtConst qtSort qtCast qtProd inductive_quotable quote_ascii bool_quotable quote_bool (*quote_string quote_positive quote_nat*) ident_quotable quote_ident quote_name nat_quotable name_quotable quote quote_term sort_quotable cast_kind_quotable quote_sort qsSet qsProp qsType universe_quotable quote_inductive qmkInd] in quote_term) in
+    quote_term t (fun x => exact x).
+  Defined.
+  Notation "‘quote’" := qquote : preterm_scope.
+End PRP.
+
 Module PP <: PretermPrimitives LC.
-  Export LC.
+  Export LC PRP.
   Definition tLambda : Preterm -> Preterm -> Preterm
     := Ast.tLambda Ast.nAnon.
   Definition qtApp : Preterm
-    := qtApp.
+    := tLambda ‘Preterm’ (tLambda ‘Preterm’ (Ast.tApp qtApp [Ast.tRel 1; (Ast.tApp qcons [‘Preterm’; Ast.tRel 0; Ast.tApp qnil [‘Preterm’]])])).
 
   Notation "‘App’" := qtApp : preterm_scope.
 
@@ -100,17 +112,20 @@ Module PP <: PretermPrimitives LC.
   Notation "‘‘VAR₀’’" := ttVar0 : well_typed_term_scope.
 End PP.
 
-Module PRP <: PretermReflectionPrimitives LC.
-  Quote Definition qPreterm := Ast.term.
-  Notation "‘Preterm’" := qPreterm : preterm_scope.
+Tactic Notation "unique" "pose" "proof" constr(defn) :=
+  let T := type of defn in
+  match goal with
+    | [ H : T |- _ ] => fail 1
+    | _ => pose proof defn
+  end.
 
-  Definition qquote : LC.Preterm.
-  Proof.
-    let t := (eval cbv beta delta [qO qS qEmptyString qString qnAnon qAscii qnil qcons qmkdef qtInd qtFix qtCase qtUnknown qtRel qtConstruct qtEvar qtMeta qtVar qtApp qtConst qtSort qtCast qtProd inductive_quotable quote_ascii bool_quotable quote_bool (*quote_string quote_positive quote_nat*) ident_quotable quote_ident quote_name nat_quotable name_quotable quote quote_term sort_quotable cast_kind_quotable quote_sort qsSet qsProp qsType universe_quotable quote_inductive qmkInd] in quote_term) in
-    quote_term t (fun x => exact x).
-  Defined.
-  Notation "‘quote’" := qquote : preterm_scope.
-End PRP.
+(** Test if a tactic succeeds, but always roll-back the results *)
+Tactic Notation "test" tactic3(tac) :=
+  try (first [ tac | fail 2 tac "does not succeed" ]; fail 0 tac "succeeds"; [](* test for [t] solved all goals *)).
+
+(** [not tac] is equivalent to [fail tac "succeeds"] if [tac] succeeds, and is equivalent to [idtac] if [tac] fails *)
+Tactic Notation "not" tactic3(tac) := try ((test tac); fail 1 tac "succeeds").
+
 
 Module TR <: TypingRules LC PP.
   Export LC PP.
@@ -120,7 +135,7 @@ Module TR <: TypingRules LC PP.
     := fun in_term new_value
        => subst_n_name in_term new_value (Some 0%nat) Ast.nAnon.
   Notation "x [ 0 ↦ y ]" := (capture_avoiding_subst_0 x y).
-  Definition convertible : Context -> Preterm -> Preterm -> Prop
+  Definition convertible : Context -> Preterm -> Preterm -> Type
     := convertible.
   Definition box'_respectful : forall {Γ A B},
                                  convertible Γ A B
@@ -130,47 +145,211 @@ Module TR <: TypingRules LC PP.
     intros Γ A B H [a Ha].
     exists a.
     eapply has_type_conv_subst; try eassumption.
+  Defined.
 
-  Axiom convertible_refl : forall {Γ}, Reflexive (convertible Γ).
-  Axiom convertible_sym : forall {Γ}, Symmetric (convertible Γ).
-  Axiom convertible_trans : forall {Γ}, Transitive (convertible Γ).
-  Axiom convertible_tApp : forall {Γ A A' B B'},
-                             convertible Γ A A'
-                             -> convertible Γ B B'
-                             -> convertible Γ (tApp A B) (tApp A' B').
-  Axiom convertible_beta_app_lambda
+  Global Instance convertible_refl : forall {Γ}, Reflexive (convertible Γ) := conv_refl.
+  Global Instance convertible_sym : forall {Γ}, Symmetric (convertible Γ) := conv_sym.
+  Global Instance convertible_trans : forall {Γ}, Transitive (convertible Γ) := conv_trans.
+  Definition convertible_beta_app_lambda
   : forall Γ A f a,
       convertible Γ (tApp (tLambda A f) a) (capture_avoiding_subst_0 f a).
-  Axiom convertible__capture_avoiding_subst_0__tApp
+  Proof.
+    intros; eapply conv_beta.
+  Defined.
+  Definition convertible__capture_avoiding_subst_0__tApp
   : forall Γ A B x,
       convertible Γ ((A ‘’ B) [ 0 ↦ x ]) ((A [ 0 ↦ x ]) ‘’ (B [ 0 ↦ x ])).
-  Axiom convertible__capture_avoiding_subst_0__qtProd
+  Proof.
+    reflexivity.
+  Defined.
+  Definition convertible__capture_avoiding_subst_0__qtProd
   : forall Γ A B x,
       convertible Γ ((A ‘‘→’’ B) [ 0 ↦ x ]) ((A [ 0 ↦ x ]) ‘‘→’’ (B [ 0 ↦ x ])).
-  Axiom convertible__capture_avoiding_subst_0__tVar0
+  Proof.
+    reflexivity.
+  Defined.
+  Definition convertible__capture_avoiding_subst_0__tVar0
   : forall Γ x,
       convertible Γ (‘VAR₀’ [ 0 ↦ x ]) x.
+  Proof.
+    reflexivity.
+  Defined.
 
-  Axiom qtProd_Proper_convertible
-  : forall Γ,
-      Proper (convertible Γ ==> convertible Γ ==> convertible Γ) qtProd.
-  Existing Instance qtProd_Proper_convertible.
-  Axiom tApp_Proper_convertible
+  Global Instance tApp_Proper_convertible
   : forall Γ,
       Proper (convertible Γ ==> convertible Γ ==> convertible Γ) tApp.
-  Existing Instance tApp_Proper_convertible.
-  Axiom convertible__quote__qtProd
+  Proof.
+    repeat intro; apply conv_tApp_respectful; assumption.
+  Defined.
+  Global Instance qtProd_Proper_convertible
+  : forall Γ,
+      Proper (convertible Γ ==> convertible Γ ==> convertible Γ) qtProd.
+  Proof.
+    repeat intro.
+    unfold qtProd.
+    apply tApp_Proper_convertible; [ | assumption ].
+    apply tApp_Proper_convertible; [ reflexivity | assumption ].
+  Defined.
+  Definition convertible__quote__qtProd
   : forall Γ A B,
       convertible Γ (⌜ A ‘→’ B ⌝) (⌜ A ⌝ ‘‘→’’ ⌜ B ⌝).
-  Axiom convertible__quote__closed
-  : forall Γ A x,
-      convertible Γ ((quote A) [ 0 ↦ x ]) (quote A).
-  Axiom convertible__qtApp__closed
+  Proof.
+    repeat intro.
+    simpl.
+    unfold qtProd, tApp; simpl.
+    symmetry.
+    apply conv_tApp_cons2.
+    apply conv_tApp_cons2.
+    reflexivity.
+  Defined.
+
+  Definition convertible__qtApp__closed
   : forall Γ x,
       convertible Γ (‘App’ [ 0 ↦ x ]) (‘App’).
-  Axiom convertible__quote__app
+  Proof.
+    reflexivity.
+  Defined.
+
+  Create HintDb t_quote_db discriminated.
+
+  Local Ltac t_quote0 tac :=
+    repeat match goal with
+             | _ => progress simpl
+             | _ => progress intros
+             | _ => reflexivity
+             | _ => apply tApp_Proper_convertible; [ solve [ tac ] | ]
+             | _ => apply tApp_Proper_convertible; [ | solve [ tac ] ]
+             | [ |- convertible _ (Ast.tApp _ (_::_::_)%list) _ ] => apply conv_tApp_cons1
+             | [ |- convertible _ _ (Ast.tApp _ (_::_::_)%list) ] => symmetry; apply conv_tApp_cons1; symmetry
+             | _ => progress change conversion.convertible with convertible
+           end.
+  Local Ltac t_quote :=
+    repeat match goal with
+             | _ => progress t_quote0 t_quote
+             | _ => solve [ eauto with nocore t_quote_db ]
+           end.
+
+  Definition convertible__quote_nat__closed_helper {Γ A x}
+  : forall n n', convertible Γ (subst_n_name (quote_nat A) x n n') (quote_nat A).
+  Proof. induction A; t_quote. Qed.
+
+  Hint Resolve convertible__quote_nat__closed_helper : t_quote_db.
+
+  Definition convertible__quote_bool__closed_helper {Γ A x}
+  : forall n n', convertible Γ (subst_n_name (quote_bool A) x n n') (quote_bool A).
+  Proof. induction A; t_quote. Qed.
+
+  Hint Resolve convertible__quote_bool__closed_helper : t_quote_db.
+
+  Definition convertible__quote_ascii__closed_helper {Γ A x}
+  : forall n n', convertible Γ (subst_n_name (quote_ascii A) x n n') (quote_ascii A).
+  Proof. induction A; t_quote. Qed.
+
+  Hint Resolve convertible__quote_ascii__closed_helper : t_quote_db.
+
+  Definition convertible__quote_ident__closed_helper {Γ A x}
+  : forall n n', convertible Γ (subst_n_name (quote_ident A) x n n') (quote_ident A).
+  Proof. induction A; t_quote. Qed.
+
+  Hint Resolve convertible__quote_ident__closed_helper : t_quote_db.
+
+  Definition convertible__quote_positive__closed_helper {Γ A x}
+  : forall n n', convertible Γ (subst_n_name (quote_positive A) x n n') (quote_positive A).
+  Proof. induction A; t_quote. Qed.
+
+  Hint Resolve convertible__quote_positive__closed_helper : t_quote_db.
+
+  Definition convertible__quote_sort__closed_helper {Γ A x}
+  : forall n n', convertible Γ (subst_n_name (quote_sort A) x n n') (quote_sort A).
+  Proof. induction A; t_quote. Qed.
+
+  Hint Resolve convertible__quote_sort__closed_helper : t_quote_db.
+
+  Definition convertible__quote_cast_kind__closed_helper {Γ A x}
+  : forall n n', convertible Γ (subst_n_name (quote_cast_kind A) x n n') (quote_cast_kind A).
+  Proof. induction A; t_quote. Qed.
+
+  Hint Resolve convertible__quote_cast_kind__closed_helper : t_quote_db.
+
+  Definition convertible__quote_name__closed_helper {Γ A x}
+  : forall n n', convertible Γ (subst_n_name (quote_name A) x n n') (quote_name A).
+  Proof. induction A; t_quote. Qed.
+
+  Hint Resolve convertible__quote_name__closed_helper : t_quote_db.
+
+  Definition convertible__quote_inductive__closed_helper {Γ A x}
+  : forall n n', convertible Γ (subst_n_name (quote_inductive A) x n n') (quote_inductive A).
+  Proof. induction A; t_quote. Qed.
+
+  Hint Resolve convertible__quote_inductive__closed_helper : t_quote_db.
+
+  Section sub_helpers.
+    Context (convertible__quote_term__closed_helper : forall (Γ : Context)
+                                                             (A x : Ast.term)
+                                                             (n : option nat)
+                                                             (n' : Ast.name),
+                                                        convertible Γ
+                                                                    (subst_n_name
+                                                                       (quote_term A) x n n')
+                                                                    (quote_term A)).
+
+    Fixpoint convertible__quote_term_helper__closed_helper Γ ls x
+    : forall n n', convertible Γ (subst_n_name (quote_term_helper quote_term ls) x n n') (quote_term_helper quote_term ls).
+    Proof.
+      destruct ls as [|y ys]; simpl; try reflexivity; [].
+      intros n n'.
+      t_quote.
+    Defined.
+
+    Fixpoint convertible__quote_term_helper_def__closed_helper Γ ls x
+    : forall n n', convertible Γ (subst_n_name (quote_term_helper_def quote_term ls) x n n') (quote_term_helper_def quote_term ls).
+    Proof.
+      destruct ls as [|[] ys]; simpl; try reflexivity; [].
+      intros n n'.
+      t_quote.
+    Defined.
+  End sub_helpers.
+
+  Fixpoint convertible__quote_term__closed_helper Γ A x {struct A}
+  : forall n n', convertible Γ (subst_n_name (quote_term A) x n n') (quote_term A).
+  Proof.
+    intros n n'; destruct A; simpl;
+    repeat match goal with
+             | [ Γ : Context, ls : list Ast.term |- _ ]
+               => unique pose proof (convertible__quote_term_helper__closed_helper convertible__quote_term__closed_helper Γ ls x n n')
+             | [ Γ : Context, ls : Ast.mfixpoint Ast.term |- _ ]
+               => unique pose proof (convertible__quote_term_helper_def__closed_helper convertible__quote_term__closed_helper Γ ls x n n')
+             | [ Γ : Context, A : Ast.term |- _ ]
+               => not constr_eq A x; unique pose proof (convertible__quote_term__closed_helper Γ A x n n')
+           end;
+    try solve [ t_quote ].
+  Defined.
+
+  Definition convertible__quote__closed
+  : forall Γ A x,
+      convertible Γ ((quote A) [ 0 ↦ x ]) (quote A).
+  Proof.
+    intros; apply convertible__quote_term__closed_helper.
+  Defined.
+
+  Hint Resolve convertible__quote__closed : t_quote_db.
+
+  Definition convertible__quote__app
   : forall Γ A B,
       convertible Γ (⌜ A ‘’ B ⌝) ((‘App’ ‘’ ⌜ A ⌝) ‘’ ⌜ B ⌝).
+  Proof.
+    intros; simpl.
+    unfold tApp, qtApp, tLambda.
+    symmetry.
+    etransitivity.
+    { apply conv_tApp_respectful; [ | reflexivity ].
+      apply conv_beta. }
+    simpl.
+    etransitivity; [ apply conv_beta | ].
+    simpl.
+    t_quote.
+  Defined.
+
 End TR.
 
 Module PRTR <: PretermReflectionTypingRules LC PP PRP TR.
